pcuic/theories/PCUICRedTypeIrrelevance.v
@@ -1,0 +1,235 @@
+From Equations Require Import Equations.
+From MetaCoq.Template Require Import config utils.
+From MetaCoq.PCUIC Require Import PCUICAst PCUICTyping PCUICLiftSubst PCUICReduction.
+
+From Coq Require Import CRelationClasses.
+
+Ltac pcuic :=
+  try repeat red; cbn in *;
+   try (solve [ intuition auto; eauto with pcuic || (try lia || congruence) ]).
+
+Lemma context_relation_nth {P n Γ Γ' d} :
+context_relation P Γ Γ' -> nth_error Γ n = Some d ->
+{ d' & ((nth_error Γ' n = Some d') *
+        let Γs := skipn (S n) Γ in
+        let Γs' := skipn (S n) Γ' in
+        context_relation P Γs Γs' *
+        P Γs Γs' d d')%type }.
+Proof.
+induction n in Γ, Γ', d |- *; destruct Γ; intros Hrel H; noconf H.
+- depelim Hrel.
+  simpl. eexists; intuition eauto.
+  eexists; intuition eauto.
+- depelim Hrel.
+  destruct (IHn _ _ _ Hrel H).
+  cbn -[skipn] in *.
+  eexists; intuition eauto.
+  destruct (IHn _ _ _ Hrel H).
+  eexists; intuition eauto.
+Qed.
+
+Lemma context_relation_nth_ass {P n Γ Γ' d} :
+context_relation P Γ Γ' -> nth_error Γ n = Some d ->
+assumption_context Γ ->
+{ d' & ((nth_error Γ' n = Some d') *
+        let Γs := skipn (S n) Γ in
+        let Γs' := skipn (S n) Γ' in
+        context_relation P Γs Γs' *
+        (d.(decl_body) = None) *
+        P Γs Γs' d d')%type }.
+Proof.
+induction n in Γ, Γ', d |- *; destruct Γ; intros Hrel H; noconf H.
+- depelim Hrel. intro ass. 
+  simpl. eexists; intuition eauto.
+  eexists; intuition eauto.
+  depelim H.
+- intros ass. depelim Hrel.
+  destruct (IHn _ _ _ Hrel H).
+  now depelim ass.
+  cbn -[skipn] in *.
+  eexists; intuition eauto.
+  destruct (IHn _ _ _ Hrel H).
+  now depelim ass.
+  eexists; intuition eauto.
+Qed.
+
+Lemma context_relation_nth_r {P n Γ Γ' d'} :
+context_relation P Γ Γ' -> nth_error Γ' n = Some d' ->
+{ d & ((nth_error Γ n = Some d) *
+        let Γs := skipn (S n) Γ in
+        let Γs' := skipn (S n) Γ' in
+        context_relation P Γs Γs' *
+        P Γs Γs' d d')%type }.
+Proof.
+induction n in Γ, Γ', d' |- *; destruct Γ'; intros Hrel H; noconf H.
+- depelim Hrel.
+  simpl. eexists; intuition eauto.
+  eexists; intuition eauto.
+- depelim Hrel.
+  destruct (IHn _ _ _ Hrel H).
+  cbn -[skipn] in *.
+  eexists; intuition eauto.
+  destruct (IHn _ _ _ Hrel H).
+  eexists; intuition eauto.
+Qed.
+
+(** Types of variables are irrelevant during reduction *)
+
+Section ContextChangeTypesReduction.
+Context {cf : checker_flags}.
+Context (Σ : global_env).
+
+Inductive change_decl_type : context_decl -> context_decl -> Type :=
+| change_vass_type : forall (na na' : aname) (T T' : term),
+    change_decl_type (vass na T) (vass na' T')
+| change_vdef_type : forall (na na' : aname) (b T T'  : term),
+    change_decl_type (vdef na b T) (vdef na' b T').
+
+Derive Signature for change_decl_type.
+
+Global Instance change_decl_type_refl : Reflexive change_decl_type.
+Proof. intros [? [|]]; constructor; reflexivity. Qed.
+
+Global Instance change_decl_type_sym : Symmetric change_decl_type.
+Proof.
+  intros x y rel.
+  depelim rel; constructor; now symmetry.
+Qed.
+
+Global Instance change_decl_type_trans : Transitive change_decl_type.
+Proof.
+  intros x y z xy yz.
+  depelim xy; depelim yz; constructor; now etransitivity.
+Qed.
+
+Global Instance change_decl_type_equiv : Equivalence change_decl_type.
+Proof. constructor; typeclasses eauto. Qed.
+
+Lemma OnOne2All_All3 {A B} (P Q : A -> B -> B -> Type) l l' l'' :
+  OnOne2All P l l' l'' ->
+  (forall x y z, P x y z -> Q x y z) ->
+  (forall x y, Q x y y) ->
+  All3 Q l l' l''.
+Proof.
+  intros H ? ?. induction H; constructor; auto.
+  induction tl in bs, e |- *; destruct bs; simpl in e; try constructor; auto; try congruence.
+Qed.
+
+Lemma context_change_decl_types_red1 Γ Γ' s t :
+  context_relation (fun _ _ => change_decl_type) Γ Γ' -> red1 Σ Γ s t -> red Σ Γ' s t.
+Proof.
+  intros HT X0. induction X0 using red1_ind_all in Γ', HT |- *; eauto.
+  all:pcuic.
+  - econstructor. econstructor.
+    rewrite <- H.
+    induction HT in i |- *; destruct i; eauto.
+    now inv p.
+  - econstructor. econstructor; eauto.
+  - eapply PCUICReduction.red_abs. eapply IHX0; eauto.  eauto.
+  - eapply PCUICReduction.red_abs. eauto. eapply IHX0. eauto.
+    eauto. econstructor. eauto. econstructor.
+  -
+    eapply PCUICReduction.red_letin. eapply IHX0; eauto.
+    all:eauto.
+  -
+    eapply PCUICReduction.red_letin; eauto.
+  -
+    eapply PCUICReduction.red_letin; eauto. eapply IHX0; eauto.
+    econstructor. eauto. econstructor.
+    
+  - eapply PCUICReduction.red_case_pars; eauto.
+    simpl. eapply OnOne2_All2; eauto. simpl. intuition auto.
+  - eapply PCUICReduction.red_case_p; eauto. eapply IHX0.
+    eapply context_relation_app_inv; auto.
+    now eapply context_relation_refl.
+  - eapply PCUICReduction.red_case_c; eauto.
+  - eapply PCUICReduction.red_case_brs; eauto.
+    eapply OnOne2All_All3; eauto. simpl.
+    intros. intuition auto. eapply b0.
+    eapply context_relation_app_inv; auto.
+    now apply context_relation_refl.
+  -
+    eapply PCUICReduction.red_proj_c. eauto.
+  -
+    eapply PCUICReduction.red_app; eauto.
+  -     eapply PCUICReduction.red_app; eauto.
+  -
+    eapply PCUICReduction.red_prod; eauto.
+  -
+    eapply PCUICReduction.red_prod; eauto. eapply IHX0. eauto. eauto.
+    econstructor.
+    eauto. econstructor. 
+  - eapply PCUICReduction.red_evar; eauto.
+    induction X; eauto. econstructor. eapply p; eauto.
+    induction tl; eauto.
+  - eapply PCUICReduction.red_fix_one_ty.
+    eapply OnOne2_impl ; eauto.
+    intros [? ? ? ?] [? ? ? ?] [[r ih] e]. simpl in *.
+    inversion e. subst. clear e.
+    split ; auto.
+  - eapply PCUICReduction.red_fix_one_body.
+    eapply OnOne2_impl ; eauto.
+    intros [? ? ? ?] [? ? ? ?] [[r ih] e]. simpl in *.
+    inversion e. subst. clear e.
+    split ; auto.
+    eapply ih ; auto.
+    clear - HT.
+    induction (fix_context mfix0) as [| [na [b|] ty] Δ ihΔ].
+    + auto.
+    + simpl. constructor ; eauto.
+      constructor. 
+    + simpl. constructor ; eauto.
+      constructor. 
+  - eapply PCUICReduction.red_cofix_one_ty.
+    eapply OnOne2_impl ; eauto.
+    intros [? ? ? ?] [? ? ? ?] [[r ih] e]. simpl in *.
+    inversion e. subst. clear e.
+    split ; auto.
+  - eapply PCUICReduction.red_cofix_one_body.
+    eapply OnOne2_impl ; eauto.
+    intros [? ? ? ?] [? ? ? ?] [[r ih] e]. simpl in *.
+    inversion e. subst. clear e.
+    split ; auto.
+    eapply ih ; auto.
+    clear - HT.
+    induction (fix_context mfix0) as [| [na [b|] ty] Δ ihΔ].
+    + auto.
+    + simpl. constructor ; eauto.
+      constructor. 
+    + simpl. constructor ; eauto.
+      constructor. 
+Qed.
+
+Lemma context_change_decl_types_red Γ Γ' s t :
+  context_relation (fun _ _ => change_decl_type) Γ Γ' -> red Σ Γ s t -> red Σ Γ' s t.
+Proof.
+  intros. induction X0 using red_rect'; eauto.
+  etransitivity. eapply IHX0.
+  eapply context_change_decl_types_red1; eauto.
+Qed.
+End ContextChangeTypesReduction.
+
+Lemma fix_context_change_decl_types Γ mfix mfix' :
+#|mfix| = #|mfix'| ->
+context_relation (fun _ _ => change_decl_type) (Γ,,, fix_context mfix) (Γ,,, fix_context mfix').
+Proof.
+intros len.
+apply context_relation_app_inv.
+- now rewrite !fix_context_length.
+- apply context_relation_refl.
+  intros.
+  destruct x.
+  destruct decl_body; constructor;
+  reflexivity.
+- unfold fix_context, mapi.
+  generalize 0 at 2 4.
+  induction mfix in mfix', len |- *; intros n.
+  + destruct mfix'; [|cbn in *; discriminate len].
+    constructor.
+  + destruct mfix'; cbn in *; [discriminate len|].
+    apply context_relation_app_inv.
+    * now rewrite !List.rev_length, !mapi_rec_length.
+    * constructor; [constructor|].
+      constructor.
+    * apply IHmfix; lia.
+Qed.
